
Let $p$ be a polynomial with natural number coefficients and degree at least two:

$$p(n) = a_d n^d + a_{d-1} n^{d-1} + \cdots + a_1 n + a_0$$

where $d \geq 2$, and $a_i \in \mathbb{N}$ for all $i$, with $a_d > 0$.

Define the language:

$$L_p = \{w \in \Sigma^* : |w| = p(n) \text{ for some } n \in \mathbb{N}\}$$

where $\Sigma$ is any non-empty alphabet and $|w|$ denotes the length of string $w$.

**Claim:** $L_p$ is not regular.

A language $L$ is regular if and only if the equivalence relation $\equiv_L$ has finitely many equivalence classes where:

$$x \equiv_L y \iff \forall z \in \Sigma^* : (xz \in L \iff yz \in L)$$


For each $n \in \mathbb{N}$, let $s_n$ be a string of length $p(n)$. That is:

$s_n = a^{p(n)}$ where $a \in \Sigma$ is any symbol.

now to show that for distinct natural numbers $m$ and $n$, the strings $s_m$ and $s_n$ are distinguishable, i.e., $s_m \not\equiv_{L_p} s_n$.

Let $m, n \in \mathbb{N}$ with $m < n$. We need to find a string $z$ such that exactly one of $s_m z$ and $s_n z$ is in $L_p$.

Since $p$ has degree $d \geq 2$ and leading coefficient $a_d > 0$ the gaps between consecutive polynomial values grow without bound. here : 

$$p(n+1) - p(n) = a_d[(n+1)^d - n^d] + a_{d-1}[(n+1)^{d-1} - n^{d-1}] + \cdots + a_1$$

For large $n$, this difference grows like $\Theta(n^{d-1})$ since:

$$(n+1)^d - n^d = dn^{d-1} + O(n^{d-2})$$

We will find a $z$ such that:
- $|s_m z| = |s_m| + |z| = p(m) + |z|$ is equal to some $p(k)$
- $|s_n z| = |s_n| + |z| = p(n) + |z|$ is NOT equal to any $p(k')$

Since $m < n$, we have $p(m) < p(n)$ (as $p$ is strictly increasing for sufficiently large arguments, and we can assume $m$ is large enough).

Choose $z$ to be a string of length:

$$|z| = p(m+1) - p(m)$$

Then:
$$|s_m z| = p(m) + [p(m+1) - p(m)] = p(m+1)$$

Therefore $s_m z \in L_p$ (since $|s_m z| = p(m+1)$).

Now we show that $s_n z \notin L_p$:

$$|s_n z| = p(n) + [p(m+1) - p(m)]$$

verifying that this length is not equal to $p(k)$ for any $k \in \mathbb{N}$.

Case 1: If $k \leq n$, then $p(k) \leq p(n) < p(n) + [p(m+1) - p(m)] = |s_n z|$ (since $p(m+1) - p(m) > 0$).

Case 2: If $k = n+1$, we need:
$$p(n) + [p(m+1) - p(m)] \neq p(n+1)$$
$$p(m+1) - p(m) \neq p(n+1) - p(n)$$

Since $m < n$ and $p$ has degree $d \geq 2$, the differences $p(i+1) - p(i)$ are strictly increasing for sufficiently large $i$ (because the derivative $p'(x)$ is a polynomial of degree $d-1 \geq 1$, which is strictly increasing).

For sufficiently large $m$ and $n$ with $m < n$:
$$p(m+1) - p(m) < p(n+1) - p(n)$$

Therefore $|s_n z| = p(n) + [p(m+1) - p(m)] < p(n) + [p(n+1) - p(n)] = p(n+1)$.

Case 3: If $k > n+1$, then $p(k) \geq p(n+2)$. We need to show:
$$p(n) + [p(m+1) - p(m)] < p(n+2)$$

This is equivalent to:
$$p(m+1) - p(m) < p(n+2) - p(n)$$

Since the gaps are increasing and $m < n$, we have:
$$p(m+1) - p(m) < p(n+1) - p(n) < p(n+2) - p(n+1)$$

And clearly:
$$p(n+2) - p(n) = [p(n+1) - p(n)] + [p(n+2) - p(n+1)] > p(n+1) - p(n) > p(m+1) - p(m)$$

Therefore, $|s_n z| = p(n) + [p(m+1) - p(m)]$ falls strictly between $p(n)$ and $p(n+1)$, so it cannot equal any polynomial value.

Thus $s_n z \notin L_p$.